Progress on prophetic proof; added forgotten wp_ResolveBytes

src/program_proof/simplepb/pb_prophetic_read.v
@@ -1,7 +1,7 @@
 From Perennial.program_proof Require Import grove_prelude.
 From Goose.github_com.mit_pdos.gokv.simplepb Require Export clerk.
 From Perennial.program_proof.simplepb Require Import pb_definitions pb_apply_proof pb_makeclerk_proof.
-From Perennial.program_proof.simplepb Require Import clerk_proof.
+From Perennial.program_proof.simplepb Require Import clerk_proof proph_proof.
 
 Section prophetic_read_proof.
 Context `{!heapGS Σ}.
@@ -17,6 +17,49 @@ Notation is_pb_Clerk := (pb_definitions.is_Clerk (pb_record:=pb_record)).
 Context `{!pbG Σ}.
 Context `{!config_proof.configG Σ}.
 
+Record proph_req_names :=
+{
+  op_gn:gname;
+  finish_gn:gname;
+}.
+
+Implicit Types γreq : proph_req_names.
+
+Context `{inG Σ dfracR}.
+
+Definition operation_incomplete γreq : iProp Σ := own γreq.(op_gn) (DfracOwn 1).
+Definition operation_receipt γreq : iProp Σ := own γreq.(op_gn) (DfracDiscarded).
+
+Lemma complete_operation γreq :
+  operation_incomplete γreq ==∗ operation_receipt γreq.
+Proof.
+  iIntros "H1".
+  iApply (own_update with "H1").
+  apply (cmra_update_exclusive).
+  done.
+Qed.
+
+Definition result_claimed γreq : iProp Σ := own γreq.(finish_gn) (DfracOwn 1).
+Definition result_unclaimed γreq : iProp Σ := own γreq.(finish_gn) (DfracOwn 1).
+
+Definition read_fupd γ readOp (Q:list u8 → iProp Σ) : iProp Σ :=
+(|={⊤∖↑pbN,∅}=> ∃ ops, own_op_log γ ops ∗
+  (own_op_log γ ops ={∅,⊤∖↑pbN}=∗ Q (compute_reply ops readOp))).
+
+Definition prophReadN := nroot .@ "prophread".
+
+Definition prophetic_read_inv prophV γ γreq readOp Φ : iProp Σ :=
+  inv prophReadN (
+        (*
+          XXX: This invariant is a bit ad-hoc. A more principled approach would be to
+          give the server a fraction of the ghost resources for the "state" of
+          this protocol at the beginning of time, and for this invariant to have
+          only a fraction of it.
+        *)
+  operation_incomplete γreq ∗ read_fupd γ readOp Φ ∨
+  operation_receipt γreq ∗ ((Φ prophV) ∨ result_claimed γreq))
+.
+
 Lemma wp_Clerk__ApplyReadonly γ ck op_sl op (op_bytes:list u8) (Φ:val → iProp Σ) :
 has_op_encoding op_bytes op →
 own_Clerk ck γ -∗
@@ -29,6 +72,48 @@ is_slice_small op_sl byteT 1 op_bytes -∗
 WP clerk.Clerk__ApplyRo #ck (slice_val op_sl) {{ Φ }}.
 Proof.
   iIntros (?) "Hck Hsl Hupd".
+  wp_call.
+  wp_apply (wp_NewProphBytes).
+  iIntros (??) "Hproph".
+  wp_pures.
+  iAssert (|={⊤}=> ∃ γreq, result_unclaimed γreq ∗ prophetic_read_inv b γ γreq _
+  (λ reply, ∀ reply_sl : Slice.t,
+             is_slice_small reply_sl byteT 1 reply -∗
+             is_slice_small op_sl byteT 1 op_bytes -∗ own_Clerk ck γ -∗ Φ (slice_val reply_sl))
+          )%I with "[Hupd]" as ">H".
+  {
+    iMod (own_alloc (DfracOwn 1)) as (γop) "Hop".
+    { done. }
+    iMod (own_alloc (DfracOwn 1)) as (γfinish) "Hfinish".
+    { done. }
+    iExists {| op_gn := γop ; finish_gn := γfinish |}.
+    iFrame. iMod (inv_alloc with "[-]") as "$"; last done.
+    iNext. iLeft. iFrame "Hop ∗".
+  }
+  iDestruct "H" as (?) "[Hfinish #Hinv]".
+  wp_bind (Clerk__ApplyRo2 _ _).
+  wp_apply (wp_frame_wand with "[Hproph Hfinish]").
+  { iNamedAccu. }
+  wp_apply (wp_Clerk__ApplyReadonly2 with "Hck Hsl []").
+  { done. }
+  iModIntro.
+  iInv "Hinv" as "Hi" "Hclose".
+  iDestruct "Hi" as "[Hnotdone|Hdone]".
+  2:{ (* case: one of the low-level uRPC requests already fired the fupd before. *)
+    iApply fupd_mask_intro.
+    { set_solver. }
+    iIntros "Hmask".
+    iRight.
+    iIntros (?) "_". iMod "Hmask".
+    iDestruct "Hdone" as "[#>? ?]".
+    iMod ("Hclose" with "[-]").
+    { iRight. iFrame "∗#". }
+    iModIntro.
+    iModIntro.
+    iIntros (?) "Hrep_sl Hop_sl Hck".
+    iNamed 1.
+    wp_pures.
+    wp_apply (wp_ResolveBytes with "Hproph").
 Qed.
 
 End prophetic_read_proof.
