src/program_proof/simplepb/proph_proof.v
@@ -25,7 +25,7 @@ Global Instance proph_bytes_timeless p b :
   Timeless (proph_once_bytes p b).
 Proof. apply _. Qed.
 
-Lemma wp_NewProphActions :
+Lemma wp_NewProphBytes :
   {{{ True }}}
     NewProph #()
   {{{ (p : proph_id) b, RET #p; proph_once_bytes p b }}}.
@@ -44,15 +44,14 @@ Proof.
 Qed.
 
 Local Lemma wp_BytesToVal sl b q :
-  {{{ is_slice sl byteT q b }}}
+  {{{ is_slice_small sl byteT q b }}}
     BytesToVal (slice_val sl)
-  {{{ v, RET v; ⌜decode_bytes v = b⌝ ∗ is_slice sl byteT q b }}}.
+  {{{ v, RET v; ⌜decode_bytes v = b⌝ ∗ is_slice_small sl byteT q b }}}.
 Proof.
   iIntros (?) "Hsl HΦ". wp_call.
   wp_apply wp_alloc_untyped. { done. }
   iIntros (l) "Hl". wp_apply (wp_store with "Hl"). iIntros "Hl". wp_pures.
-  iDestruct (is_slice_sz with "Hsl") as %Hsz.
-  iDestruct (is_slice_split with "Hsl") as "[Hsl Hc]".
+  iDestruct (is_slice_small_sz with "Hsl") as %Hsz.
   wp_apply (wp_forSlice (λ i, ∃ b' v, ⌜decode_bytes v = b' ∧ b' = take (int.nat i) b⌝ ∗ l ↦ v)%I
     with "[] [Hl $Hsl]").
   2:{ iExists [], _. iFrame. iPureIntro. done. }
@@ -75,6 +74,26 @@ Proof.
   wp_pures. wp_apply (wp_load with "Hl"). iIntros "Hl".
   iApply "HΦ". iFrame. iPureIntro. destruct H as [? ?].
   subst. rewrite H0. rewrite firstn_all2; first done. word.
+Qed.
+
+Lemma wp_ResolveBytes sl p b b' q :
+  {{{ proph_once_bytes p b' ∗ is_slice_small sl byteT q b }}}
+    ResolveBytes #p (slice_val sl)
+  {{{ RET #(); ⌜b' = b⌝ ∗ is_slice_small sl byteT q b }}}.
+Proof.
+  iIntros (?) "[Hproph ?] HΦ".
+  wp_call.
+  wp_apply (wp_BytesToVal with "[$]").
+  iIntros (?) "[% ?]".
+  wp_pures.
+  iDestruct "Hproph" as (?) "[? %]".
+  wp_apply (wp_resolve_proph with "[$]").
+  iIntros (?) "[% _]".
+  iApply "HΦ".
+  iFrame.
+  iPureIntro.
+  subst.
+  done.
 Qed.
 End proph.
 
